\documentclass{article}
\input{../cfg/preamble}
\title{5.7 Differential Equations}

\begin{document}
    \maketitle
    \textbf{Introduction}\\
    Given an unknown equation $ y $ 

    Suppouse $ y'=Ay $, can we solve for $ y $?

    \[
        \begin{gathered}
        \begin{bmatrix}
            a &b\\
            c &d
        \end{bmatrix}
        \begin{bmatrix}
            y_1\\
            y)2
        \end{bmatrix}=
        \begin{bmatrix}
            y'_1\\
            y'_2
        \end{bmatrix}
        \end{gathered}
    \]

    \[
        \begin{gathered}
        ay_1+by_2=y'_1\\
        cy_1+dy_2=y'_2
        \end{gathered}
    \]

    Consider the differential equation,
    \[
        \begin{gathered}
        Dy=y'\\
        ~\\
        \begin{bmatrix}
            \lambda_1 &0\\
            0 &\lambda_2
        \end{bmatrix}
        \begin{bmatrix}
            y_1\\
            y_2
        \end{bmatrix}=
        \begin{bmatrix}
            y'_1\\
            y'_2
        \end{bmatrix}
        \end{gathered}
    \]

    We can see that
    \[
        \begin{gathered}
        \lambda_1 y_1=y'_1\\
        \lambda_2 y_2=y'_2
        \end{gathered}
    \]

    Now that this is decoupled, we can get
    \[
        \begin{gathered}
            \lambda_1 y_1=y'_1 \to y_1=e^{\lambda_1 x}+C_1\\
            \lambda_2 y_2=y'_2 \to y_2=e^{\lambda_2 x}+C_2 
        \end{gathered}
    \]

    \textbf{Ex 1}\\
    Solve $ x'=Ax $
    \[
        \begin{gathered}
        \begin{bmatrix}
            x_1'(t)\\
            x'_2(t)
        \end{bmatrix}=
        \begin{bmatrix}
            3 &0\\
            0 &-5
        \end{bmatrix}
        \begin{bmatrix}
            x_1(t)\\
            x_2(t)
        \end{bmatrix}\\
        ~\\
        x_1(t)=e^{3t}+C_1\\
        x_2(t)=e^{-5t}+C_2  
        \end{gathered}
    \]

    \textbf{Ex 2}\\
    Solve $ x'=Ax $, where $ A=\begin{bmatrix}
        -1.5 &0.5\\
        1 &-1
    \end{bmatrix} $ and $ x(0)=\begin{bmatrix}
        5\\
        4
    \end{bmatrix} $ 

    Firstly, find the eigenvalues of $ A $ and solve $ \text{det}(A-\lambda I) =0$ in order to diagonalize $ A $.
    \[
        \begin{gathered}
        \begin{bmatrix}
        -1.5 - \lambda &0.5\\
        1 &-1-\lambda
        \end{bmatrix}
        \end{gathered}=0
    \]

    So
    \[
        \begin{gathered}
          (\lambda + 1.5)(\lambda + 1)-0.5=0\\
          \lambda^{2} + 2.5\lambda + 1=0\\
          ~\\
          \lambda_1 = -0.5 \qquad \lambda_2 = -2 
        \end{gathered}
    \]

    Then we solve for the eigenvectors $ v_1 ~\&~ v_2 $
    \[
        \begin{gathered}
        \lambda_1=-0.5
        \begin{bmatrix}
            -1 &0.5 &0\\
            1 &-0.5 &0
        \end{bmatrix}\\
        v_1=\begin{bmatrix}
            1\\
            2
        \end{bmatrix}\\
        ~\\
        \lambda_2 = -2\\
        \begin{bmatrix}
            0.5 &0.5 &0\\
            1 &1 &0
        \end{bmatrix}\\
        v_2=\begin{bmatrix}
            -1\\
            1
        \end{bmatrix}
        \end{gathered}
    \]

    The general solution of $ x'=\begin{bmatrix}
        -1.5 &0.5\\
        1 &-1
    \end{bmatrix}x $ is
    \[
        \begin{gathered}
        x(t)=\begin{bmatrix}
            x_1(t)\\
            x_2(t)
        \end{bmatrix}=c_1v_1e^{\lambda_1 t} + c_2v_2 e^{\lambda_2 t}\\
        c_1 \begin{bmatrix}
            1\\
            2
        \end{bmatrix}e^{-\frac{1}{2}t}+c_2\begin{bmatrix}
            -1\\
            1
        \end{bmatrix} e^{-2t}  
        \end{gathered}
    \]
    
\end{document}
