\documentclass{article}
\input{../cfg/preamble}
\title{11.5 Chain Rule}

\begin{document}
  \maketitle
  \textbf{Introduction}\\
  There are several versions of the Chain Rule for multi variable functions. Each of these versions give a rule for differentiating a composite functions.

  \textbf{Chain Rule Case 11}\\
  $ z=f(x,y) $ with $ x,y =g(t),h(t) $, meaning that $ x ~\&~ y $ are both functions of $ t $. Then $ z $ is a differentiable function of $ t $. Assume that $ f_{x} ~\&~ f_{y}   $ are continuous so $ f $ is differentiable.  
  \[
    \begin{gathered}
    z=f(x,y),~x=g(t),~y=h(t)\\
    ~\\
    \frac{dz}{dt} = z_{x} \frac{dx}{dx} + z_{y}\frac{dy}{dt} =  \frac{\partial z}{\partial x} \frac{dx}{dt}+\frac{\partial z}{\partial y} \frac{dy}{dt} 
    ~\\
    \end{gathered}
  \]

  \textbf{Ex 1}\\
  If $ z=x^{2}y+3xy^{4} $, where $ x=\sin{2t} ~\&~ y=\cos{t}$, find $ \frac{dz}{dt} $ when $ t=0 $.
  \[
    \begin{gathered}
    \frac{\partial z}{\partial x} = 2xy+3y^{4},~\frac{dx}{dt} =2\cos{2t} \qquad \frac{\partial z}{\partial x}=x^{2}+12xy^{3},~\frac{dy}{i}=-\sin{t}\\
    ~\\
    \frac{dz}{dt} = (2xy+3y^{3} )(2\cos{2t})+(x^{2}+12x^{3} )(-\sin{t})\\
    ~\\
    t=0,~x=\sin{0}=0,~y=\cos{0}=1\\
    ~\\
  \frac{dz}{dt} |_{t=0} =(0+3)(2\cdot 1)+(0+0)(-\sin{0})=\boxed{6}
    \end{gathered}
  \]

  \textbf{Ex 2}\\
  $ PV =8.31T$. Find the rate at which the pressure is changing when the temperature is $ 300K $ and increasing at a rate of $ 0.1K/s $ and the volume is $ 100L $ and ijncreasing at a rate of $ 0.2L/s $.
  \[
    \begin{gathered}
    T=300, \frac{dT}{dt}=0.1,~V=100,~\frac{dV}{dt}=0.2\\
    ~\\
    P=8.31\frac{T}{V} \\
    ~\\
  \frac{dP}{dt}= P_{T}\frac{dT}{dt}+ P_{v}\frac{dV}{dt} = \frac{\partial P}{\partial T} \frac{dT}{dt}+\frac{\partial P}{\partial V} \frac{dV}{dt}\\
  ~\\
  \frac{\partial}{\partial T}= 8.31\frac{T}{V},~\frac{dT}{dt}= 0.1  \qquad \frac{\partial P}{\partial V}=-2\frac{8.31T}{v^{2} },~\frac{dV}{dt} =0.2\\
  ~\\
  \frac{dP}{dt} = 0.1 (\frac{8.31}{100}) -0.2(\frac{8.31(300)}{100^{2}})=\boxed{-0.04155}\\
  ~\\
  \text{The pressure is decreasing at a rate of about } 0.042kPa/s  
    \end{gathered}
  \]
 
  \textbf{Chain Rule Case 2}\\
  Suppouse that $ z=f(x,y) $ is a differentiable function of $ x ~\&~ y $, where $ x=g(s,t) ~\&~ y=h(s,t)$ are differentiable functions of $ s ~\&~ t $. Then
  \[
    \begin{gathered}
    \frac{\partial z}{\partial s} = z_{x}x_{s}+z_{y}y_{s} = \frac{\partial z}{\partial x} \frac{\partial x}{\partial s} +\frac{\partial z}{\partial y} \frac{\partial y}{\partial s}\\
    ~\\
    \frac{\partial z}{\partial t} = z_{x} x_{t}+z_{y}y_{t} = \frac{\partial z}{\partial x} \frac{\partial x}{\partial t} + \frac{\partial z}{\partial y} \frac{\partial y}{\partial t}    
    \end{gathered}
  \]

  \textbf{Ex 3}\\
  If $ z=e^{x}\sin{y} $, where $ x=st^{2}  ~\&~ y=s^{2}t $, find $ \frac{\partial z}{\partial s} ~\&~ \frac{\partial z}{\partial t}  $.
  \[
    \begin{gathered}
      \frac{\partial z}{\partial s}:= \qquad \frac{\partial z}{\partial x}=e^{x}\sin{y},~\frac{\partial x}{\partial s}=t^{2},~\frac{\partial z}{\partial y}=e^{x}\cos{y},~\frac{\partial y}{\partial s}=2st\\
    \frac{\partial z}{\partial s}= t^{2} e^{x}\sin{y} )+2ste^{x}\cos{y}\\
    \boxed{\frac{\partial z}{\partial s} = t^{2}e^{st^{2}}\sin{(s^{2}t)} + 2st e^{st^{2} }\cos{(s^{2}t)}}\\
    ~\\
    ~\\
    \frac{\partial z}{\partial s} := \qquad \frac{\partial z}{\partial x}=e^{x}\sin{y},~\frac{\partial x}{\partial t}=2ts,~\frac{\partial z}{\partial y}=e^{x}\cos{y},~\frac{\partial y}{\partial t}=s^{2}\\
    \frac{\partial z}{\partial s}=2ste^{x}\sin{y}+s^{2}e^{x}\cos{y}\\
    \boxed{\frac{\partial z}{\partial s}= 2ste^{st^{2}}\sin{(st^{2})}+s^{2}e^{st^{2}}\cos{(s^{2}t)}}      
    \end{gathered}
  \]
  
  \textbf{General Version}\\
  Suppouse that $ u $ is a differentiable function of the $ n $ variables $ x_{1},x_{2},...,x_{n} $ and each $ x_{i}  $ is a differentiable function of the $ m $ variables $ t_{1},t_{2},...,t_{m} $.
  \[
      \begin{gathered}
      \frac{\partial u}{\partial t_{i} } = \frac{\partial u}{\partial x_{1} } \frac{\partial x_{1} }{\partial t_{j} }+\frac{\partial u}{\partial x_{2} }\frac{\partial x_{2}}{\partial t_{j}}+...+\frac{\partial u}{\partial x_{n} }\frac{\partial x_{n} }{\partial t_{m} }
      \end{gathered}
  \]
  for each $ j =1,2,...,m$.

  \textbf{Ex 4}\\
  If $ u=x^{4}y+y^{2}z^{3}    $, where $ =rse^{t},y=rs^{2}e^{-t}, ~\&~ z=r^{2}s\sin{t}$, find $ \frac{\partial u}{\partial s} $.
  \[
      \begin{gathered}
      \frac{\partial u}{\partial s} = \frac{\partial u}{\partial x}\frac{\partial x}{\partial s}+\frac{\partial u}{\partial y}\frac{\partial y}{\partial s}+\frac{\partial u}{\partial z}\frac{\partial z}{\partial s}\\
      ~\\
      \boxed{\frac{\partial u}{\partial s}=(4x^{3} y)(re^{t})+(x^{4}+2yz^{3} )(2rse^{-t})+(3y^{2}z^{2}  )(r^{2}\sin{t})} 
      \end{gathered}
  \]

    \textbf{Implicit Differentiation}\\
    Suppouse an equation of the form $ F(x,y)=0 $ defines $ y $ implicity as a differentiable function of $ x $.

    If $ F $ is differentiable and $ \frac{\partial F}{\partial y} \neq 0 $, then
    \[
        \frac{dy}{dx}=-\frac{Fx}{Fy} 
    \]

    \textbf{Ex 5}
    Find $ y'$ if $ x^{3}+y^{3}=6xy$, $ F(x,y)=x^{3}+y^{3}-6xy=0 $
    \[
        \begin{gathered}
          F_{x}=3x^{2}-6y \qquad F_{y}=3y^{2}-6x\\
          ~\\
          y'=-\frac{3x^{2}-6y}{3y^{2}-6x}=\boxed{- \frac{x^{2}-2y }{y^{2}-2x }}  
        \end{gathered}
    \]

    Suppouse $ z $ is given implicitly as $ z=f(x,y)$ by an equation of the form $ F(x,y,z)=0 $. If $ F ~\&~ f $ are differentiable and $ \frac{\partial F}{\partial Z}\neq 0 $, then
    \[
        \begin{gathered}
        \frac{\partial z}{\partial x}= -\frac{\partial F_{x} }{\partial F_{z} } \qquad \frac{\partial z}{\partial y}=-\frac{F_{y} }{F_{z}} 
        \end{gathered}
    \]

    \textbf{Ex 6}\\
    Find $ \frac{dz}{dx}  $ if $ x^{3}+y^{3}+z^{3}+6xzy=1   $
    \[
        \begin{gathered}
        F(x,y,z)=x^{3}+y^{3}+6xy-1=0\\
        ~\\
        F_{x}=3x^{2}+6yz \qquad F_{z}=3z^{2}+6xy\\
        ~\\
        \frac{dz}{dx}=- \frac{3x^{2}+6yz}{3z^{2}+6xy} = \boxed{- \frac{x^{2+2yz} }{z^{2}+2xy}} 
        \end{gathered}
    \]
\end{document}
