\documentclass{article}
\input{../cfg/preamble}
\title{11.3 Derivatives}

\begin{document}
  \maketitle
  \textbf{Notations}\\
  If $ \zstroke = f(x,y), $
  \[
    \begin{gathered}
    f_{x}(x,y)=f_{x}=\frac{df}{dx}=\frac{d}{dx} f(x,y)\\
    f_{y}(x,y)=f_{y}=\frac{df}{dy}=\frac{d}{y} f(x,y)\\
    \frac{dz}{dy},~ f_{2},~,~D_{2}f,~D_{y}f    
    \end{gathered}
  \]

  \textbf{Rules for Finding Partial Derivatives}\\
  1) To find $ f_{x} $, regard $ y $ as a constant and differentiate $ f(x,y) $ with respect to x.

  2) To find $ f_{y}  $, regard $ y $ as a constant and differentiate $ f(x,y) $ with respect to y.

  \textbf{Ex 1}\\
  If $ f(x,y) =x^{3}+x^{2}y^{3}-2y^{2}    $, find $ f_{x}(2,1) ~\&~ f_{y}(2,1)$.
  \[
    \begin{gathered}
      f_{x}(x,y)= \frac{d}{dx}x^{3}+\frac{d}{dx}(x^{2}y^{3})-\frac{d}{dx}{2y^{2}}\\
      ~\\
      3x^{2}+  y^{3} \cdot \frac{d}{dx}x^{2}-0\to 3x^{2}+2xy^{3}\\
      ~\\
      f_{x}(2,1) = 3(2)^{2} + 2(2)(1)^{3}\to \boxed{16}\\
      ~\\
      f_{y}(x,y)= \frac{d}{dy}x^{3}+\frac{d}{dy}(x^{2}y^{3})-\frac{d}{dy}2y^{2}.      
    \end{gathered}
  \]
  
   
\end{document}
